LogicGenerator/demo931/Interface.v
@@ -1,0 +1,140 @@
+Require Import Coq.Numbers.BinNums.
+Require Import Coq.PArith.BinPosDef.
+Require Import Logic.lib.PTree.
+Require Import Coq.Sets.Ensembles.
+Require Import Coq.Lists.List.
+Import ListNotations.
+
+Module Type LanguageSig.
+(* primitive_types *)
+  Parameter model : Type .
+(* derived types *)
+  Definition expr := (model -> Prop) .
+(* primitive judgements *)
+(* primitive connectives *)
+  Parameter join : (model -> model -> model -> Prop) .
+End LanguageSig.
+
+Module DerivedNames (Names: LanguageSig).
+Include Names.
+(* derived connectives *)
+  Definition impp := (fun (x y : model -> Prop) (m : model) => x m -> y m) .
+  Definition sepcon := (fun (x y : model -> Prop) (m : model) => exists m1 m2 : model, join m1 m2 m /\ x m1 /\ y m2) .
+(* derived judgements *)
+  Definition provable := (fun x : model -> Prop => forall m : model, x m) .
+End DerivedNames.
+
+Module Type PrimitiveRuleSig (Names: LanguageSig).
+Include DerivedNames (Names).
+  Axiom join_comm : (forall m1 m2 m : model, join m1 m2 m -> join m2 m1 m) .
+  Axiom join_assoc : (forall mx my mz mxy mxyz : model, join mx my mxy -> join mxy mz mxyz -> exists myz : model, join my mz myz /\ join mx myz mxyz) .
+End PrimitiveRuleSig.
+
+Module Type LogicTheoremSig (Names: LanguageSig) (Rules: PrimitiveRuleSig Names).
+Include Rules.
+Parameter Inline tree_pos : Type .
+(* derived rules *)
+  Axiom sepcon_comm_impp : (forall x y : expr, provable (impp (sepcon x y) (sepcon y x))) .
+  Axiom sepcon_assoc1 : (forall x y z : expr, provable (impp (sepcon x (sepcon y z)) (sepcon (sepcon x y) z))) .
+  Axiom sepcon_mono : (forall x1 x2 y1 y2 : expr, provable (impp x1 x2) -> provable (impp y1 y2) -> provable (impp (sepcon x1 y1) (sepcon x2 y2))) .
+  Axiom sepcon_comm_impp : (forall x y : expr, provable (impp (sepcon x y) (sepcon y x))) .
+  Axiom sepcon_assoc1 : (forall x y z : expr, provable (impp (sepcon x (sepcon y z)) (sepcon (sepcon x y) z))) .
+  Axiom sepcon_mono : (forall x1 x2 y1 y2 : expr, provable (impp x1 x2) -> provable (impp y1 y2) -> provable (impp (sepcon x1 y1) (sepcon x2 y2))) .
+  Axiom sepcon_proper_impp : (Morphisms.Proper (Morphisms.respectful (fun x y : expr => provable (impp x y)) (Morphisms.respectful (fun x y : expr => provable (impp x y)) (fun x y : expr => provable (impp x y)))) sepcon) .
+  Axiom expr_deep : Set .
+  Axiom impp_deep : (expr_deep -> expr_deep -> expr_deep) .
+  Axiom sepcon_deep : (expr_deep -> expr_deep -> expr_deep) .
+  Axiom emp_deep : expr_deep .
+  Axiom varp_deep : (nat -> expr_deep) .
+  Axiom var_pos : (expr -> option positive -> tree_pos) .
+  Axiom sepcon_pos : (tree_pos -> tree_pos -> tree_pos) .
+  Axiom cancel_mark : (expr_deep -> expr_deep -> tree_pos -> tree_pos -> tree_pos * tree_pos) .
+  Axiom cancel_same : (tree_pos -> tree_pos -> Prop) .
+  Axiom restore : (tree_pos -> tree_pos -> expr) .
+(* derived rules as instance *)
+  Existing Instance sepcon_proper_impp .
+End LogicTheoremSig.
+
+Require Import Logic.GeneralLogic.Base.
+Require Import Logic.GeneralLogic.ProofTheory.BasicSequentCalculus.
+Require Import Logic.GeneralLogic.ProofTheory.BasicDeduction.
+Require Import Logic.MinimumLogic.Syntax.
+Require Import Logic.MinimumLogic.ProofTheory.Minimum.
+Require Import Logic.MinimumLogic.ProofTheory.RewriteClass.
+Require Import Logic.MinimumLogic.ProofTheory.TheoryOfJudgement.
+Require Import Logic.PropositionalLogic.Syntax.
+Require Import Logic.PropositionalLogic.ProofTheory.Intuitionistic.
+Require Import Logic.PropositionalLogic.ProofTheory.DeMorgan.
+Require Import Logic.PropositionalLogic.ProofTheory.GodelDummett.
+Require Import Logic.PropositionalLogic.ProofTheory.Classical.
+Require Import Logic.PropositionalLogic.ProofTheory.RewriteClass.
+Require Import Logic.PropositionalLogic.ProofTheory.ProofTheoryPatterns.
+Require Import Logic.PropositionalLogic.ProofTheory.TheoryOfIteratedConnectives.
+Require Import Logic.PropositionalLogic.ProofTheory.TheoryOfClassicalAxioms.
+Require Import Logic.PropositionalLogic.ProofTheory.TheoryOfPropositionalConnectives.
+Require Import Logic.MetaLogicInj.Syntax.
+Require Import Logic.MetaLogicInj.ProofTheory.ProofRules.
+Require Import Logic.SeparationLogic.Syntax.
+Require Import Logic.SeparationLogic.ProofTheory.SeparationLogic.
+Require Import Logic.SeparationLogic.ProofTheory.RewriteClass.
+Require Import Logic.SeparationLogic.ProofTheory.DerivedRules.
+Require Import Logic.SeparationLogic.ProofTheory.TheoryOfCancel.
+Require Import Logic.SeparationLogic.ProofTheory.TheoryOfSeparationAxioms.
+Require Import Logic.SeparationLogic.ProofTheory.IterSepcon.
+Require Import Logic.SeparationLogic.ProofTheory.Corable.
+Require Import Logic.SeparationLogic.ProofTheory.Deduction.
+Require Import Logic.GeneralLogic.ProofTheory.BasicLogicEquiv.
+Require Import Logic.SeparationLogic.Model.SeparationAlgebra.
+Require Import Logic.SeparationLogic.ShallowEmbedded.Join2Sepcon.
+Require Import Logic.GeneralLogic.ShallowEmbedded.PredicateAsLang.
+Require Import Logic.SeparationLogic.ShallowEmbedded.PredicateSeparationLogic.
+
+Module LogicTheorem (Names: LanguageSig) (Rules: PrimitiveRuleSig Names) <: LogicTheoremSig Names Rules.
+Include Rules.
+(* aux primitive instances *)
+  Instance M : Model := (Build_Model model) .
+  Instance L : Language := (Build_Language expr) .
+  Instance J : (Join model) := join .
+  Instance minL : (MinimumLanguage L) := (Build_MinimumLanguage L impp) .
+  Instance sepconL : (SepconLanguage L) := (Build_SepconLanguage L sepcon) .
+  Instance GammaP : (Provable L) := (Build_Provable L provable) .
+  Instance J_SA : (SeparationAlgebra model) := (Build_SeparationAlgebra model J join_comm join_assoc) .
+(* aux refl instances for derivation *)
+  Instance imppDef_model : (ImppDefinition_Model minL_modelL) := Model2Impp_Normal .
+  Instance sepconFJ : (SepconDefinition_Join Join2Sepcon) := Join2Sepcon_Normal .
+  Instance provableDef_model : (ProvableDefinition_Model GammaP_modelL) := Model2Provable_Normal .
+(* aux derived instances *)
+  Instance sepconAX_modelL : (SepconAxiomatization Model_L GammaP_modelL) := SeparationAlgebra2SepconAxiomatization .
+Definition tree_pos : Type := tree_pos.
+(* derived rules *)
+  Definition sepcon_comm_impp : (forall x y : expr, provable (impp (sepcon x y) (sepcon y x))) := sepcon_comm_impp .
+  Definition sepcon_assoc1 : (forall x y z : expr, provable (impp (sepcon x (sepcon y z)) (sepcon (sepcon x y) z))) := sepcon_assoc1 .
+  Definition sepcon_mono : (forall x1 x2 y1 y2 : expr, provable (impp x1 x2) -> provable (impp y1 y2) -> provable (impp (sepcon x1 y1) (sepcon x2 y2))) := sepcon_mono .
+  Definition sepcon_comm_impp : (forall x y : expr, provable (impp (sepcon x y) (sepcon y x))) := sepcon_comm_impp .
+  Definition sepcon_assoc1 : (forall x y z : expr, provable (impp (sepcon x (sepcon y z)) (sepcon (sepcon x y) z))) := sepcon_assoc1 .
+  Definition sepcon_mono : (forall x1 x2 y1 y2 : expr, provable (impp x1 x2) -> provable (impp y1 y2) -> provable (impp (sepcon x1 y1) (sepcon x2 y2))) := sepcon_mono .
+  Definition sepcon_proper_impp : (Morphisms.Proper (Morphisms.respectful (fun x y : expr => provable (impp x y)) (Morphisms.respectful (fun x y : expr => provable (impp x y)) (fun x y : expr => provable (impp x y)))) sepcon) := sepcon_proper_impp .
+  Definition expr_deep : Set := expr_deep .
+  Definition impp_deep : (expr_deep -> expr_deep -> expr_deep) := impp_deep .
+  Definition sepcon_deep : (expr_deep -> expr_deep -> expr_deep) := sepcon_deep .
+  Definition emp_deep : expr_deep := emp_deep .
+  Definition varp_deep : (nat -> expr_deep) := varp_deep .
+  Definition var_pos : (expr -> option positive -> tree_pos) := var_pos .
+  Definition sepcon_pos : (tree_pos -> tree_pos -> tree_pos) := sepcon_pos .
+  Definition cancel_mark : (expr_deep -> expr_deep -> tree_pos -> tree_pos -> tree_pos * tree_pos) := cancel_mark .
+  Definition cancel_same : (tree_pos -> tree_pos -> Prop) := cancel_same .
+  Definition restore : (tree_pos -> tree_pos -> expr) := restore .
+(* derived rules as instance *)
+  Existing Instance sepcon_proper_impp .
+End LogicTheorem.
+
+(*Require Logic.PropositionalLogic.DeepEmbedded.Solver.
+Module IPSolver (Names: LanguageSig).
+  Import Names.
+  Ltac ip_solve :=
+    change expr with Base.expr;
+    change provable with Base.provable;
+    change impp with Syntax.impp;
+    change andp with Syntax.andp;
+    intros; Solver.SolverSound.ipSolver.
+End IPSolver.*)
